changed implicit arguments of lhs_fun_defined

trunk/color/DP/ADPUnif.v
@@ -14,133 +14,140 @@ Require Import ADecomp AUnif ARenCap ATrs ListUtil RelUtil AGraph LogicUtil
 
 Section S.
 
-Variable N : nat. (* maximum number of unification steps *)
+  Variable N : nat. (* maximum number of unification steps *)
 
 (***********************************************************************)
 (** over graph based on unification *)
 
-Section unif.
+  Section unif.
 
-Variable Sig : Signature.
+    Variable Sig : Signature.
 
-Notation rule := (rule Sig). Notation rules := (rules Sig).
+    Notation rule := (rule Sig). Notation rules := (rules Sig).
 
-Variables R D : rules.
+    Variables R D : rules.
 
-Definition connectable u v := unifiable (ren_cap R (S (maxvar v)) u) v.
+    Definition connectable u v := unifiable (ren_cap R (S (maxvar v)) u) v.
 
-Definition dpg_unif (r1 r2 : rule) :=
-  In r1 D /\ In r2 D /\ connectable (rhs r1) (lhs r2).
+    Definition dpg_unif (r1 r2 : rule) :=
+      In r1 D /\ In r2 D /\ connectable (rhs r1) (lhs r2).
 
-Variable hypR : forallb (@is_notvar_lhs Sig) R = true.
+    Variable hypR : forallb (@is_notvar_lhs Sig) R = true.
 
-Lemma dpg_unif_correct : hd_rules_graph (red R #) D << dpg_unif.
+    Lemma dpg_unif_correct : hd_rules_graph (red R #) D << dpg_unif.
 
-Proof.
-intros x y h. destruct h. decomp H0. unfold dpg_unif. intuition.
-destruct x as [l1 r1]. destruct y as [l2 r2]. simpl in *.
-unfold connectable. set (k := S (maxvar l2)).
-destruct (rtc_red_sub_ren_cap hypR k H2). destruct (ren_cap_sub R x1 r1 k).
-destruct H3. gen H0. rewrite H3. unfold shift. repeat rewrite sub_sub. intro.
-assert (forall x, In x (vars (ren_cap R k r1)) -> In x (vars l2) -> False).
-intros. ded (vars_ren_cap H5). ded (vars_max H6). subst k. omega.
-unfold unifiable. eapply sub_eq_is_sol. hyp. symmetry in H0. apply H0.
-Qed.
+    Proof.
+      intros x y h. destruct h. decomp H0. unfold dpg_unif. intuition.
+      destruct x as [l1 r1]. destruct y as [l2 r2]. simpl in *.
+      unfold connectable. set (k := S (maxvar l2)).
+      destruct (rtc_red_sub_ren_cap hypR k H2).
+      destruct (ren_cap_sub R x1 r1 k).
+      destruct H3. gen H0. rewrite H3. unfold shift. repeat rewrite sub_sub.
+      intro. assert (forall x, In x (vars (ren_cap R k r1))
+        -> In x (vars l2) -> False).
+      intros. ded (vars_ren_cap H5). ded (vars_max H6). subst k. omega.
+      unfold unifiable. eapply sub_eq_is_sol. hyp. symmetry in H0. apply H0.
+    Qed.
 
 (***********************************************************************)
 (** over graph using a finite number of unification steps *)
 
-Definition ren_cap (r1 r2 : rule) := ren_cap R (S (maxvar (lhs r2))) (rhs r1).
+    Definition ren_cap (r1 r2 : rule) :=
+      ren_cap R (S (maxvar (lhs r2))) (rhs r1).
 
-Definition unifiable_N r1 r2 :=
-  iter_step N (mk_problem (ren_cap r1 r2) (lhs r2)).
+    Definition unifiable_N r1 r2 :=
+      iter_step N (mk_problem (ren_cap r1 r2) (lhs r2)).
 
-Require Import AHDE.
+    Require Import AHDE.
 
-Definition connectable_N r1 r2 :=
-  match unifiable_N r1 r2 with
-  | None => false
-  | Some (_, nil) => true
-  | _ => hd_eq (rhs r1) (lhs r2)
-  end.
+    Definition connectable_N r1 r2 :=
+      match unifiable_N r1 r2 with
+        | None => false
+        | Some (_, nil) => true
+        | _ => hd_eq (rhs r1) (lhs r2)
+      end.
 
-Notation mem := (mem (@beq_rule Sig)).
-Notation mem_ok := (mem_ok (@beq_rule_ok Sig)).
+    Notation mem := (mem (@beq_rule Sig)).
+    Notation mem_ok := (mem_ok (@beq_rule_ok Sig)).
 
-Definition dpg_unif_N r1 r2 := mem r1 D && mem r2 D && connectable_N r1 r2.
+    Definition dpg_unif_N r1 r2 := mem r1 D && mem r2 D && connectable_N r1 r2.
 
-Variable hypD : forallb (undefined_rhs R) D = true.
+    Variable hypD : forallb (undefined_rhs R) D = true.
 
-Lemma successfull_hd_eq : forall x r1 r2, In r1 D -> In r2 D ->
-  successfull (iter_step x (mk_problem (ren_cap r1 r2) (lhs r2))) = true ->
-  hd_eq (rhs r1) (lhs r2) = true.
+    Lemma successfull_hd_eq : forall x r1 r2, In r1 D -> In r2 D ->
+      successfull (iter_step x (mk_problem (ren_cap r1 r2) (lhs r2))) = true ->
+      hd_eq (rhs r1) (lhs r2) = true.
 
-Proof.
-intros x r1 r2 h1 h2 H. set (p := mk_problem (ren_cap r1 r2) (lhs r2)) in H.
-assert (problem_wf p). apply wf_mk_problem. destruct (successfull_is_sol H0 H).
-gen H1. unfold p, mk_problem, ren_cap. simpl. intuition. gen H1.
-rewrite forallb_forall in hypD. ded (hypD _ h1). ded (hypD _ h2).
-destruct r1 as [l1 r1]. destruct r2 as [l2 r2]. simpl. destruct r1. refl.
-destruct l2. refl. set (k := S (maxvar (Fun f0 v0))). rewrite ren_cap_fun.
-gen H1. unfold undefined_rhs, undefined. simpl. rewrite negb_lr. simpl. intro.
-rewrite H1. unfold is_sol_eqn. unfold fst, snd. repeat rewrite sub_fun.
-intro. Funeqtac. rewrite H6. rewrite (beq_refl (@beq_symb_ok Sig)). refl.
-Qed.
+    Proof.
+      intros x r1 r2 h1 h2 H.
+      set (p := mk_problem (ren_cap r1 r2) (lhs r2)) in H.
+      assert (problem_wf p). apply wf_mk_problem.
+      destruct (successfull_is_sol H0 H).
+      gen H1. unfold p, mk_problem, ren_cap. simpl. intuition. gen H1.
+      rewrite forallb_forall in hypD. ded (hypD _ h1). ded (hypD _ h2).
+      destruct r1 as [l1 r1]. destruct r2 as [l2 r2]. simpl. destruct r1. refl.
+      destruct l2. refl. set (k := S (maxvar (Fun f0 v0))). rewrite ren_cap_fun.
+      gen H1. unfold undefined_rhs, undefined. simpl. rewrite negb_lr. simpl.
+      intro. rewrite H1. unfold is_sol_eqn. unfold fst, snd.
+      repeat rewrite sub_fun. intro. Funeqtac. rewrite H6.
+      rewrite (beq_refl (@beq_symb_ok Sig)). refl.
+    Qed.
 
-Lemma dpg_unif_N_correct : hd_rules_graph (red R #) D << Graph dpg_unif_N.
+    Lemma dpg_unif_N_correct : hd_rules_graph (red R #) D << Graph dpg_unif_N.
 
-Proof.
-trans dpg_unif. apply dpg_unif_correct. intros r1 r2 h. destruct h.
-destruct H0. unfold Graph, dpg_unif_N. rewrite <- mem_ok in H.
-rewrite <- mem_ok in H0. rewrite H. rewrite H0. bool.
-destruct (iter_step_complete (wf_mk_problem (ren_cap r1 r2) (lhs r2)) H1).
-unfold connectable_N, unifiable_N. case (lt_eq_lt_dec x N); intro. destruct s.
-ded (successfull_preserved H2 l). destruct (successfull_elim H3). rewrite H4.
-refl. subst. destruct (successfull_elim H2). rewrite H3. refl.
-ded (successfull_inv H2 l).
-destruct (iter_step N (mk_problem (ren_cap r1 r2) (lhs r2))). 2: irrefl.
-destruct p. destruct e. refl. eapply successfull_hd_eq.
-rewrite <- mem_ok. hyp. rewrite <- mem_ok. hyp. apply H2.
-Qed.
+    Proof.
+      trans dpg_unif. apply dpg_unif_correct. intros r1 r2 h. destruct h.
+      destruct H0. unfold Graph, dpg_unif_N. rewrite <- mem_ok in H.
+      rewrite <- mem_ok in H0. rewrite H. rewrite H0. bool.
+      destruct (iter_step_complete (wf_mk_problem (ren_cap r1 r2) (lhs r2)) H1).
+      unfold connectable_N, unifiable_N. case (lt_eq_lt_dec x N); intro.
+      destruct s. ded (successfull_preserved H2 l).
+      destruct (successfull_elim H3). rewrite H4.
+      refl. subst. destruct (successfull_elim H2). rewrite H3. refl.
+      ded (successfull_inv H2 l).
+      destruct (iter_step N (mk_problem (ren_cap r1 r2) (lhs r2))). 2: irrefl.
+      destruct p. destruct e. refl. eapply successfull_hd_eq.
+      rewrite <- mem_ok. hyp. rewrite <- mem_ok. hyp. apply H2.
+    Qed.
 
-End unif.
+  End unif.
 
 (***********************************************************************)
 (** with marked symbols *)
 
-Section mark.
+  Section mark.
 
-Variable Sig : Signature.
+    Variable Sig : Signature.
 
-Notation Sig' := (dup_sig Sig).
+    Notation Sig' := (dup_sig Sig).
 
-Lemma undefined_hd_symb_dup_int_rules : forall f R,
-  @defined Sig' (hd_symb Sig f) (dup_int_rules R) = false.
+    Lemma undefined_hd_symb_dup_int_rules : forall f R,
+      @defined Sig' (hd_symb Sig f) (dup_int_rules R) = false.
 
-Proof.
-induction R; intros. refl. simpl dup_int_rules. destruct a as [l r].
-destruct l; hyp.
-Qed.
+    Proof.
+      induction R; intros. refl. simpl dup_int_rules. destruct a as [l r].
+      destruct l; hyp.
+    Qed.
 
-Variables R D : rules Sig.
+    Variables R D : rules Sig.
 
-Notation R' := (dup_int_rules R). Notation D' := (dup_hd_rules D).
+    Notation R' := (dup_int_rules R). Notation D' := (dup_hd_rules D).
 
-Variable hypR : forallb (@is_notvar_lhs Sig') R' = true.
-Variable hypD : forallb (@is_notvar_rhs Sig') D' = true.
+    Variable hypR : forallb (@is_notvar_lhs Sig') R' = true.
+    Variable hypD : forallb (@is_notvar_rhs Sig') D' = true.
 
-Lemma dpg_unif_N_mark_correct :
-  hd_rules_graph (red R' #) D' << Graph (dpg_unif_N R' D').
+    Lemma dpg_unif_N_mark_correct :
+      hd_rules_graph (red R' #) D' << Graph (dpg_unif_N R' D').
 
-Proof.
-apply dpg_unif_N_correct. hyp. rewrite forallb_forall. intros.
-unfold undefined_rhs. destruct (in_map_elim H). destruct H0. subst.
-destruct x0 as [l r]. simpl. unfold undefined. destruct r.
-rewrite forallb_forall in hypD. ded (hypD _ H). discr. simpl.
-rewrite negb_lr. apply undefined_hd_symb_dup_int_rules.
-Qed.
+    Proof.
+      apply dpg_unif_N_correct. hyp. rewrite forallb_forall. intros.
+      unfold undefined_rhs. destruct (in_map_elim H). destruct H0. subst.
+      destruct x0 as [l r]. simpl. unfold undefined. destruct r.
+      rewrite forallb_forall in hypD. ded (hypD _ H). discr. simpl.
+      rewrite negb_lr. apply undefined_hd_symb_dup_int_rules.
+    Qed.
 
-End mark.
+  End mark.
 
 End S.
 
